
\documentclass[12pt]{article}
\usepackage{graphicx}
\usepackage[fleqn]{amsmath}  % fleqn : left-align
\usepackage{braket}


\begin{document}

\section{5.1. Quantum Fourier transform}

\subsection{5.12}

If the first bit is $\ket{0}$:

\begin{equation*}
\begin{aligned}
&
H \cdot (\ket{0}) 
= 
\frac{1}{\sqrt{2}}
\begin{pmatrix}
1 & 1 \\ 
1 & -1 
\end{pmatrix}
(\ket{0})
= 
\frac{1}{\sqrt{2}}
\begin{pmatrix}
1 & 1 \\ 
1 & -1 
\end{pmatrix}
\begin{pmatrix}
1 \\ 
0 
\end{pmatrix}
=
\frac{1}{\sqrt{2}}
\begin{pmatrix}
1 \\ 
1 
\end{pmatrix} \\
&=
\frac{1}{\sqrt{2}}
(\ket{0} + \ket{1})
= 
\frac{1}{\sqrt{2}}
(\ket{0} + e^{2\pi i 0} \ket{1})
\end{aligned}
\end{equation*}

%------------------

If the first bit is $\ket{1}$:

\begin{equation*}
\begin{aligned}
&
H \cdot (\ket{1}) 
= 
\frac{1}{\sqrt{2}}
\begin{pmatrix}
1 & 1 \\ 
1 & -1 
\end{pmatrix}
(\ket{1})
= 
\frac{1}{\sqrt{2}}
\begin{pmatrix}
1 & 1 \\ 
1 & -1 
\end{pmatrix}
\begin{pmatrix}
0 \\ 
1 
\end{pmatrix}
=
\frac{1}{\sqrt{2}}
\begin{pmatrix}
1 \\ 
-1 
\end{pmatrix} \\
&=
\frac{1}{\sqrt{2}}
(\ket{0} - \ket{1})
= 
\frac{1}{\sqrt{2}}
(\ket{0} + e^{2\pi i \frac{1}{2}} \ket{1})
\end{aligned}
\end{equation*}

because $e^{i\pi} = -1$.

\end{document}
