
\documentclass[12pt]{article}
\usepackage{graphicx}
\usepackage[fleqn]{amsmath}  % fleqn : left-align


\begin{document}

\begin{equation*}
\mbox{Let} \qquad \alpha = 1/ \sqrt{2}
\end{equation*}

%----------------------------------------%

\section{Eig(X)}

\begin{equation*}
\begin{aligned}
| I - \lambda X |
=
\left|
\begin{pmatrix}
1 & 0 \\ 
0 & 1 
\end{pmatrix}
- \lambda
\begin{pmatrix}
0 & 1 \\ 
1 & 0 
\end{pmatrix}
\right|
=
\begin{vmatrix}
1 & -\lambda \\ 
-\lambda & 1 
\end{vmatrix}
= 1 - \lambda^2
\Rightarrow
\lambda = \pm 1
\end{aligned}
\end{equation*}

% X, lambda = 1

\begin{equation*}
\begin{aligned}
Xv & = 1 \cdot v \Leftrightarrow 
\begin{pmatrix}
0 & 1 \\ 
1 & 0 
\end{pmatrix}
\begin{pmatrix}
a \\ 
b 
\end{pmatrix}
=
\begin{pmatrix}
a \\ 
b 
\end{pmatrix}
\Leftrightarrow 
\begin{cases}
b = a \\
a = b
\end{cases}
\rightarrow
v = 
\alpha
\begin{pmatrix}
1 \\ 
1 
\end{pmatrix}
\end{aligned}
\end{equation*}

% X, lambda = -1

\begin{equation*}
\begin{aligned}
Xv & = 1 \cdot v \Leftrightarrow 
\begin{pmatrix}
0 & 1 \\ 
1 & 0 
\end{pmatrix}
\begin{pmatrix}
a \\ 
b 
\end{pmatrix}
=
- \begin{pmatrix}
a \\ 
b 
\end{pmatrix}
\Leftrightarrow 
\begin{cases}
b = -a \\
a = -b
\end{cases}
\rightarrow
v = 
\alpha
\begin{pmatrix}
1 \\ 
-1 
\end{pmatrix}
\end{aligned}
\end{equation*}

%----------------------------------------%

\section{Eig(Y)}

\begin{equation*}
\begin{aligned}
| I - \lambda Y |
=
\left|
\begin{pmatrix}
1 & 0 \\ 
0 & 1 
\end{pmatrix}
- \lambda
\begin{pmatrix}
0 & -i \\ 
i & 0 
\end{pmatrix}
\right|
=
\begin{vmatrix}
1 & \lambda i \\ 
-\lambda i & 1 
\end{vmatrix}
= 1 - \lambda^2
\Rightarrow
\lambda = \pm 1
\end{aligned}
\end{equation*}

% Y, lambda = 1

\begin{equation*}
\begin{aligned}
Yv & = 1 \cdot v \Leftrightarrow 
\begin{pmatrix}
0 & -i \\ 
i & 0 
\end{pmatrix}
\begin{pmatrix}
a \\ 
b 
\end{pmatrix}
=
\begin{pmatrix}
a \\ 
b 
\end{pmatrix}
\Leftrightarrow 
\begin{cases}
-ib = a \\
ia = b
\end{cases}
\rightarrow
v = 
\alpha
\begin{pmatrix}
1 \\ 
i 
\end{pmatrix}
\end{aligned}
\end{equation*}

% Y, lambda = -1

\begin{equation*}
\begin{aligned}
Yv & = 1 \cdot v \Leftrightarrow 
\begin{pmatrix}
0 & -i \\ 
i & 0 
\end{pmatrix}
\begin{pmatrix}
a \\ 
b 
\end{pmatrix}
=
- \begin{pmatrix}
a \\ 
b 
\end{pmatrix}
\Leftrightarrow 
\begin{cases}
-ib = -a \\
ia = -b
\end{cases}
\rightarrow
v = 
\alpha
\begin{pmatrix}
1 \\ 
-i 
\end{pmatrix}
\end{aligned}
\end{equation*}

%----------------------------------------%

\section{Eig(Z)}

\begin{equation*}
\begin{aligned}
| I - \lambda Z |
=
\left|
\begin{pmatrix}
1 & 0 \\ 
0 & 1 
\end{pmatrix}
- \lambda
\begin{pmatrix}
1 & 0 \\ 
0 & -1 
\end{pmatrix}
\right|
=
\begin{vmatrix}
1 -\lambda & 0 \\ 
0 & 1 + \lambda 
\end{vmatrix}
\Rightarrow
\lambda = \pm 1
\end{aligned}
\end{equation*}

% Z, lambda = 1

\begin{equation*}
\begin{aligned}
Zv & = 1 \cdot v \Leftrightarrow 
\begin{pmatrix}
1 & 0 \\ 
0 & -1 
\end{pmatrix}
\begin{pmatrix}
a \\ 
b 
\end{pmatrix}
=
\begin{pmatrix}
a \\ 
b 
\end{pmatrix}
\Leftrightarrow 
\begin{cases}
a = a \\
-b = b
\end{cases}
\rightarrow
v = 
\begin{pmatrix}
1 \\ 
0
\end{pmatrix}
\end{aligned}
\end{equation*}

% Z, lambda = -1

\begin{equation*}
\begin{aligned}
Zv & = 1 \cdot v \Leftrightarrow 
\begin{pmatrix}
1 & 0 \\ 
0 & -1 
\end{pmatrix}
\begin{pmatrix}
a \\ 
b 
\end{pmatrix}
=
- \begin{pmatrix}
a \\ 
b 
\end{pmatrix}
\Leftrightarrow 
\begin{cases}
a = -a \\
-b = -b
\end{cases}
\rightarrow
v = 
\begin{pmatrix}
0 \\ 
1 
\end{pmatrix}
\end{aligned}
\end{equation*}

%----------------------------------------%

\section{Eig(H)}

\begin{equation*}
\begin{aligned}
| I - \lambda H |
& =
\left|
\begin{pmatrix}
1 & 0 \\ 
0 & 1 
\end{pmatrix}
- \lambda \alpha
\begin{pmatrix}
1 & 1 \\ 
1 & -1 
\end{pmatrix}
\right|
=
\begin{vmatrix}
1 - \alpha \lambda & - \alpha \lambda \\ 
- \alpha \lambda & 1 + \alpha \lambda 
\end{vmatrix} \\
& =
1 - (\alpha \lambda)^2  - (\alpha \lambda)^2 = 1 - \lambda^2
\Rightarrow
\lambda = \pm 1
\end{aligned}
\end{equation*}

% H, lambda = 1

\begin{equation*}
\begin{aligned}
Hv & = 1 \cdot v \Leftrightarrow 
\alpha
\begin{pmatrix}
1 & 1 \\ 
1 & -1 
\end{pmatrix}
\begin{pmatrix}
a \\ 
b 
\end{pmatrix}
=
\begin{pmatrix}
a \\ 
b 
\end{pmatrix}
\Leftrightarrow 
\begin{cases}
\alpha (a + b) = a \\
\alpha (a - b) = b
\end{cases} \\
& \rightarrow
v = 
\begin{pmatrix}
1 \\ 
\sqrt{2} - 1
\end{pmatrix}
\end{aligned}
\end{equation*}

% H, lambda = -1

\begin{equation*}
\begin{aligned}
Hv & = 1 \cdot v \Leftrightarrow 
\alpha 
\begin{pmatrix}
1 & 1 \\ 
1 & -1 
\end{pmatrix}
\begin{pmatrix}
a \\ 
b 
\end{pmatrix}
=
- \begin{pmatrix}
a \\ 
b 
\end{pmatrix}
\Leftrightarrow 
\begin{cases}
\alpha (a + b) = -a \\
\alpha (a - b) = -b
\end{cases} \\
& \rightarrow
v = 
\begin{pmatrix}
1 \\ 
\sqrt{2} + 1 
\end{pmatrix}
\end{aligned}
\end{equation*}



\end{document}
